prove permutations_fact, additions0_left

words.v
@@ -1,6 +1,34 @@
 Require Import List Permutation Factorial Arith.
-Require Import Lia.
+Require Import Lia Setoid.
 Import ListNotations.
+
+Section flat_map.
+(* TODO: remove when https://github.com/coq/coq/pull/17082 is released *)
+Lemma concat_length A l:
+  length (concat l) = list_sum (map (@length A) l).
+Proof.
+  induction l; [reflexivity|].
+  simpl. rewrite app_length.
+  f_equal. assumption.
+Qed.
+
+Lemma flat_map_length A B (f: A -> list B) l:
+  length (flat_map f l) = list_sum (map (fun x => length (f x)) l).
+Proof.
+  rewrite flat_map_concat_map, concat_length, map_map. reflexivity.
+Qed.
+
+Corollary flat_map_constant_length A B c (f: A -> list B) l:
+  (forall x, In x l -> length (f x) = c) -> length (flat_map f l) = (length l) * c.
+Proof.
+  intro H. rewrite flat_map_length.
+  induction l; [reflexivity|].
+  simpl. rewrite IHl, H.
+  - reflexivity.
+  - left. reflexivity.
+  - intros x Hx. apply H. right. assumption.
+Qed.
+End flat_map.
 
 Section factorials.
 Fixpoint falling_fact n x :=
@@ -65,44 +93,79 @@ Proof.
   - rewrite H. constructor.
 Qed.
 
-Fixpoint insert_all0 x (left right: list A) :=
+Fixpoint additions0 x (left right: list A) :=
 match right with
 | nil => [left++[x]]
-| y::right' => (left++x::right)::(insert_all0 x (left++[y]) right')
+| y::right' => (left++x::right)::(additions0 x (left++[y]) right')
 end.
 
-Definition insert_all x l := insert_all0 x nil l.
+Definition additions x l := additions0 x nil l.
 
-Lemma insert_all0_length_left x l:
-  forall left, length (insert_all0 x left l) = length (insert_all x l).
+Lemma additions0_length_left x l:
+  forall left, length (additions0 x left l) = length (additions x l).
 Proof.
   induction l.
   - reflexivity.
   - intro left. cbn. rewrite !IHl. reflexivity.
-Qed. 
+Qed.
+
+Lemma additions0_left x l:
+  forall left, In (left ++ l) (additions0 x left l) <-> In l (additions x l).
+Proof. (* TODO: redo *)
+  induction l.
+  - intro left. cbn. split; intros [].
+    + apply app_inv_head in H. left. assumption.
+    + contradiction H.
+    + left. f_equal. assumption.
+    + contradiction H.
+  - intro left. split; intro H.
+    + cbn in *. destruct H.
+      * left. apply app_inv_head in H. assumption.
+      * right. apply (IHl [a0]). specialize (IHl (left ++ [a0])).
+        replace ((left ++ [a0]) ++ l) with (left ++ a0 :: l) in IHl.
+        -- apply IHl in H. assumption.
+        -- rewrite app_assoc_reverse. reflexivity.
+    + right. specialize (IHl (left ++ [a0])) as H1.
+      replace ((left ++ [a0]) ++ l) with (left ++ a0 :: l) in H1.
+      * apply H1. specialize (IHl [a0]). cbn in *. destruct H.
+        -- exfalso. apply f_equal with (f := @length _) in H.
+           cbn in H. injection H. clear. apply Nat.neq_succ_diag_l.
+        -- apply IHl. assumption.
+      * rewrite app_assoc_reverse. reflexivity.
+Qed.
+
+Lemma insert_all_in x (l1 l2: list A):
+  In (l1++x::l2) (additions x (l1++l2)).
+Proof.
+  revert l2. induction l1.
+  - destruct l2; left; reflexivity.
+  - intros. right. cbn. 
+Abort.
 
 Lemma Add_insert_all x:
-  forall (l l': list A), Add x l l' <-> In l' (insert_all x l).
+  forall (l l': list A), Add x l l' <-> In l' (additions x l).
 Proof.
   intros l l'. split; intro H.
   - induction H.
     + destruct l; left; reflexivity.
     + apply Add_split in H. destruct H as [l1 [l2 [-> ->]]].
-      cbn. right. 
+      right. induction l1.
+      * destruct l2; left; reflexivity.
+      * right. cbn. cbn in IHl1.
 Abort. 
 
-Lemma insert_all_length x l:
-  length (insert_all x l) = S (length l).
+Lemma additions_length x l:
+  length (additions x l) = S (length l).
 Proof.
-  unfold insert_all. induction l.
+  unfold additions. induction l.
   - reflexivity.
-  - cbn. f_equal. rewrite insert_all0_length_left in *. assumption.
+  - cbn. f_equal. rewrite additions0_length_left in *. assumption.
 Qed.
 
 Fixpoint permutations l :=
 match l with
 | nil => [[]]
-| x::l' => flat_map (insert_all x) (permutations l')
+| x::l' => flat_map (additions x) (permutations l')
 end.
 
 Lemma permutations_spec:
@@ -112,6 +175,16 @@ Proof.
   - induction H.
     + left. reflexivity.
     + apply in_flat_map. exists l'.
-Abort.
+Admitted.
+
+Theorem permutations_fact l:
+  length (permutations l) = fact (length l).
+Proof.
+  induction l.
+  - reflexivity.
+  - cbn. rewrite flat_map_constant_length with (c := S (length l)); [lia|].
+    intros x Hx%permutations_spec. rewrite additions_length.
+    f_equal. apply Permutation_length. symmetry. assumption.
+Qed.
 
 End permutations.
